Refactoring Set, renaming, simplifying elt methods in Circuit

src/Circuit.fst
@@ -1,12 +1,13 @@
 ﻿(** Reversible circuit data type & utilities *)
 module Circuit
 
-(* Reversible circuit data structure & utilities. Properties proven
+open FStar.Set
+open SetExtra
+open Total
+
+(* Reversible circuit data structure & utilities.Properties proven
    mainly involve which bits may be modified by a circuit, and that
    various methods of uncomputing a computation are correct *)
-
-open Set
-open Total
 
 type gate =
   | RCNOT of int * int
@@ -15,18 +16,15 @@ type gate =
 
 type circuit = list gate
 
-val prettyPrintGate    : gate -> string
-val prettyPrintCircuit : circuit -> list string
+val prettyPrintGate    : gate -> Tot string
+val prettyPrintCircuit : circuit -> Tot (list string)
 
 val applyGate          : state -> gate -> Tot state
 val evalCirc           : circuit -> state -> Tot state
 val wfGate             : gate -> Tot bool
 val wfCirc             : circuit -> Tot bool
-val used               : int -> circuit -> Tot bool
 val uses               : circuit -> Tot (set int)
-val modded             : int -> circuit -> Tot bool
 val mods               : circuit -> Tot (set int)
-val ctrl               : int -> circuit -> Tot bool
 val ctrls              : circuit -> Tot (set int)
 val uncompute          : circuit -> int -> Tot circuit
 
@@ -42,7 +40,7 @@ let prettyPrintGate gate = match gate with
                       (String.strcat " " (Prims.string_of_int c)))))
   | RNOT a -> String.strcat "tof " (Prims.string_of_int a)
 
-let prettyPrintCircuit = List.map prettyPrintGate
+let prettyPrintCircuit = FStar.List.Tot.map prettyPrintGate
 
 (* Evaluation *)
 let applyGate st gate = match gate with
@@ -65,37 +63,34 @@ let rec wfCirc circ = match circ with
   | x::xs -> wfGate x && wfCirc xs
 
 (* Uses, targets, and controls. Uses mods and ctrls are highly inefficient *)
-let rec used i lst = match lst with
-  | [] -> false
-  | (RCNOT (a, b))::xs    -> a = i || b = i || used i xs
-  | (RTOFF (a, b, c))::xs -> a = i || b = i || c = i || used i xs
-  | (RNOT a)::xs          -> a = i || used i xs
-let uses lst = fun i -> used i lst
+let rec uses lst = match lst with
+  | []                   -> empty
+  | (RCNOT (a, b))::xs    -> ins a (ins b (uses xs))
+  | (RTOFF (a, b, c))::xs -> ins a (ins b (ins c (uses xs)))
+  | (RNOT a)::xs          -> ins a (uses xs)
 
-let rec modded i gates = match gates with
-  | [] -> false
+let rec mods gates = match gates with
+  | []                   -> empty
   | (RCNOT (_, t))::xs
   | (RTOFF (_, _, t))::xs
-  | (RNOT t)::xs -> i = t || modded i xs
-let mods gates = fun i -> modded i gates
+  | (RNOT t)::xs          -> ins t (mods xs)
 
-let rec ctrl i lst = match lst with
-  | [] -> false
-  | (RCNOT (a, b))::xs    -> a = i || ctrl i xs
-  | (RTOFF (a, b, c))::xs -> a = i || b = i || ctrl i xs
-  | (RNOT a)::xs          -> ctrl i xs
-let ctrls gates = fun i -> ctrl i gates
+let rec ctrls lst = match lst with
+  | []                   -> empty
+  | (RCNOT (a, _))::xs    -> ins a (ctrls xs)
+  | (RTOFF (a, b, _))::xs -> ins a (ins b (ctrls xs))
+  | (RNOT _)::xs          -> ctrls xs
 
 (* Uncompute relative a target bit *)
 let rec uncompute circ targ = match circ with
   | [] -> []
-  | x::xs -> if (used targ [x]) then uncompute xs targ else x::(uncompute xs targ)
+  | x::xs -> if (mem targ (uses [x])) then uncompute xs targ else x::(uncompute xs targ)
 
 (** Verification utilities *)
 
 (* Lemmas about modified bits *)
 val ref_imp_use : gates:circuit ->
-  Lemma (forall i. modded i gates \/ ctrl i gates <==> used i gates)
+  Lemma (Set.equal (uses gates) (union (mods gates) (ctrls gates)))
 let rec ref_imp_use gates = match gates with
   | [] -> ()
   | x::xs -> ref_imp_use xs
@@ -113,7 +108,9 @@ val apply_mod : st:state -> x:gate ->
 let apply_mod st x = ()
 
 val eval_mod : st:state -> gates:circuit ->
-  Lemma (agree_on st (evalCirc gates st) (complement (mods gates))) (decreases gates)
+  Lemma (requires True)
+	(ensures (agree_on st (evalCirc gates st) (complement (mods gates))))
+  (decreases gates)
 let rec eval_mod st gates = match gates with
   | [] -> ()
   | x::xs -> apply_mod st x; eval_mod (applyGate st x) xs
@@ -128,50 +125,29 @@ let rec evalCirc_append l1 l2 st = match l1 with
   | [] -> ()
   | x::xs -> evalCirc_append xs l2 (applyGate st x)
 
-val use_append : i:int -> x:circuit -> y:circuit ->
-  Lemma (requires true)
-        (ensures  (used i (x@y) <==> used i x \/ used i y))
-  [SMTPat (used i (x@y))]
-let rec use_append i x y = match x with
-  | [] -> ()
-  | x::xs -> use_append i xs y
-
 val uses_append : x:circuit -> y:circuit ->
-  Lemma (requires true)
-        (ensures  (uses (x@y) = union (uses x) (uses y)))
+  Lemma (requires True)
+        (ensures (Set.equal (uses (x@y)) (union (uses x) (uses y))))
   [SMTPat (uses (x@y))]
-let rec uses_append x y =
-  lemma_equal_intro (uses (x@y)) (union (uses x) (uses y))
-
-val mod_append : i:int -> l1:circuit -> l2:circuit ->
-  Lemma (requires true)
-        (ensures  (modded i (l1@l2) <==> modded i l1 \/ modded i l2))
-  [SMTPat (modded i (l1@l2))]
-let rec mod_append i l1 l2 = match l1 with
+let rec uses_append x y = match x with
   | [] -> ()
-  | x::xs -> mod_append i xs l2
+  | x::xs -> uses_append xs y
 
 val mods_append : x:circuit -> y:circuit ->
-  Lemma (requires true)
-        (ensures  (mods (x@y) = union (mods x) (mods y)))
+  Lemma (requires True)
+        (ensures  (Set.equal (mods (x@y)) (union (mods x) (mods y))))
   [SMTPat (mods (x@y))]
-let rec mods_append x y =
-  lemma_equal_intro (mods (x@y)) (union (mods x) (mods y))
-
-val ctrl_append : i:int -> x:circuit -> y:circuit ->
-  Lemma (requires true)
-        (ensures  (ctrl i (x@y) <==> ctrl i x \/ ctrl i y))
-  [SMTPat (ctrl i (x@y))]
-let rec ctrl_append i x y = match x with
+let rec mods_append x y = match x with
   | [] -> ()
-  | x::xs -> ctrl_append i xs y
+  | x::xs -> mods_append xs y
 
 val ctrls_append : x:circuit -> y:circuit ->
-  Lemma (requires true)
-        (ensures  (ctrls (x@y) = union (ctrls x) (ctrls y)))
+  Lemma (requires True)
+        (ensures  (Set.equal (ctrls (x@y)) (union (ctrls x) (ctrls y))))
   [SMTPat (ctrls (x@y))]
-let rec ctrls_append x y =
-  lemma_equal_intro (ctrls (x@y)) (union (ctrls x) (ctrls y))
+let rec ctrls_append x y = match x with
+  | [] -> ()
+  | x::xs -> ctrls_append xs y
 
 val wf_append : x:circuit -> y:circuit ->
   Lemma (requires (wfCirc x /\ wfCirc y))
@@ -183,57 +159,57 @@ let rec wf_append x y = match x with
 
 (* Lemmas about reversibility *)
 val rev_uses : circ:circuit ->
-  Lemma (requires true)
-        (ensures (uses circ = uses (List.rev circ)))
-  [SMTPat (uses (List.rev circ))]
+  Lemma (requires True)
+        (ensures (Set.equal (uses circ) (uses (FStar.List.Tot.rev circ))))
+  [SMTPat (uses (FStar.List.Tot.rev circ))]
 let rec rev_uses circ = match circ with
   | [] -> ()
   | x::xs ->
-    ListProperties.rev_append [x] xs;
+    FStar.ListProperties.rev_append [x] xs;
     rev_uses xs;
-    lemma_equal_intro (uses circ) (uses (List.rev circ))
+    lemma_equal_intro (uses circ) (uses (FStar.List.Tot.rev circ))
 
 val rev_mods : circ:circuit ->
-  Lemma (requires true)
-        (ensures (mods circ = mods (List.rev circ)))
-  [SMTPat (mods (List.rev circ))]
+  Lemma (requires True)
+        (ensures (Set.equal (mods circ) (mods (FStar.List.Tot.rev circ))))
+  [SMTPat (mods (FStar.List.Tot.rev circ))]
 let rec rev_mods circ = match circ with
   | [] -> ()
   | x::xs ->
-    ListProperties.rev_append [x] xs;
+    FStar.ListProperties.rev_append [x] xs;
     rev_mods xs;
-    lemma_equal_intro (mods circ) (mods (List.rev circ))
+    lemma_equal_intro (mods circ) (mods (FStar.List.Tot.rev circ))
 
 val rev_ctrls : circ:circuit ->
-  Lemma (requires true)
-        (ensures (ctrls circ = ctrls (List.rev circ)))
-  [SMTPat (ctrls (List.rev circ))]
+  Lemma (requires True)
+        (ensures (Set.equal (ctrls circ) (ctrls (FStar.List.Tot.rev circ))))
+  [SMTPat (ctrls (FStar.List.Tot.rev circ))]
 let rec rev_ctrls circ = match circ with
   | [] -> ()
   | x::xs ->
-    ListProperties.rev_append [x] xs;
+    FStar.ListProperties.rev_append [x] xs;
     rev_ctrls xs;
-    lemma_equal_intro (ctrls circ) (ctrls (List.rev circ))
+    lemma_equal_intro (ctrls circ) (ctrls (FStar.List.Tot.rev circ))
 
 val evalCirc_append_rev : x:circuit -> y:circuit -> st:state ->
-  Lemma (evalCirc (List.rev (x@y)) st = evalCirc (List.rev x) (evalCirc (List.rev y) st))
-let evalCirc_append_rev x y st = ListProperties.rev_append x y
+  Lemma (evalCirc (FStar.List.Tot.rev (x@y)) st = evalCirc (FStar.List.Tot.rev x) (evalCirc (FStar.List.Tot.rev y) st))
+let evalCirc_append_rev x y st = FStar.ListProperties.rev_append x y
 
 val rev_gate : gate:gate -> st:state ->
   Lemma (requires (wfGate gate))
-        (ensures  (Equal (applyGate (applyGate st gate) gate) st))
+        (ensures  (equal (applyGate (applyGate st gate) gate) st))
 let rev_gate gate st = lemma_map_equal_intro (applyGate (applyGate st gate) gate) st
 
 val rev_inverse : circ:circuit -> st:state ->
   Lemma (requires (wfCirc circ))
-        (ensures  (Equal (evalCirc (circ@(List.rev circ)) st) st))
+        (ensures  (equal (evalCirc (circ@(FStar.List.Tot.rev circ)) st) st))
 let rec rev_inverse circ st = match circ with
   | [] -> ()
   | x::xs ->
     rev_inverse xs (applyGate st x);
     evalCirc_append_rev [x] xs (evalCirc xs (applyGate st x));
     rev_gate x st;
-    lemma_map_equal_intro (evalCirc (circ@(List.rev circ)) st) st
+    lemma_map_equal_intro (evalCirc (circ@(FStar.List.Tot.rev circ)) st) st
 
 val applyGate_state_swap : x:gate -> st:state -> st':state -> dom:set int ->
   Lemma (requires (subset (ctrls [x]) dom /\ agree_on st st' dom))
@@ -252,17 +228,17 @@ let rec evalCirc_state_swap circ st st' dom = match circ with
 (* Lemmas for uncomputing after copying to a target *)
 val bennett : comp:circuit -> copy:circuit -> st:state ->
   Lemma (requires (wfCirc comp /\ disjoint (uses comp) (mods copy)))
-        (ensures  (agree_on st (evalCirc (comp@copy@(List.rev comp)) st) (uses comp)))
+        (ensures  (agree_on st (evalCirc (comp@copy@(FStar.List.Tot.rev comp)) st) (uses comp)))
 let bennett comp copy st =
   let st'   = evalCirc comp st in
   let st''  = evalCirc copy st' in
     eval_mod st' copy;
-    ctrls_sub_uses (List.rev comp);
-    evalCirc_state_swap (List.rev comp) st' st'' (uses comp);
+    ctrls_sub_uses (FStar.List.Tot.rev comp);
+    evalCirc_state_swap (FStar.List.Tot.rev comp) st' st'' (uses comp);
     rev_inverse comp st
 
 val uncompute_targ : circ:circuit -> targ:int ->
-  Lemma (not (modded targ (uncompute circ targ)))
+  Lemma (not (mem targ (mods (uncompute circ targ))))
 let rec uncompute_targ circ targ = match circ with
   | [] -> ()
   | x::xs -> uncompute_targ xs targ
@@ -290,14 +266,14 @@ let rec uncompute_ctrls_subset circ targ = match circ with
   | x::xs -> uncompute_ctrls_subset xs targ
 
 val uncompute_agree : circ:circuit -> targ:int -> st:state ->
-  Lemma (requires (wfCirc circ /\ not (ctrl targ circ)))
+  Lemma (requires (wfCirc circ /\ not (mem targ (ctrls circ))))
         (ensures  (agree_on (evalCirc circ st)
                             (evalCirc (uncompute circ targ) st)
                             (complement (singleton targ))))
 let rec uncompute_agree circ targ st = match circ with
   | [] -> ()
   | x::xs ->
-    if (used targ [x])
+    if (mem targ (uses [x]))
     then
       (evalCirc_state_swap xs (applyGate st x) st (complement (singleton targ));
        uncompute_agree xs targ st;
@@ -309,17 +285,17 @@ let rec uncompute_agree circ targ st = match circ with
 
 
 val uncompute_mixed_inverse : circ:circuit -> targ:int -> st:state ->
-  Lemma (requires (wfCirc circ /\ not (ctrl targ circ)))
-        (ensures  (agree_on st (evalCirc (List.rev (uncompute circ targ))
+  Lemma (requires (wfCirc circ /\ not (mem targ (ctrls circ))))
+        (ensures  (agree_on st (evalCirc (FStar.List.Tot.rev (uncompute circ targ))
                                          (evalCirc circ st))
                                (complement (singleton targ))))
 let uncompute_mixed_inverse circ targ st =
   uncompute_agree circ targ st;
   uncompute_ctrls_subset circ targ;
-  evalCirc_state_swap (List.rev (uncompute circ targ))
+  evalCirc_state_swap (FStar.List.Tot.rev (uncompute circ targ))
                       (evalCirc circ st)
                       (evalCirc (uncompute circ targ) st)
                       (complement (singleton targ));
   rev_inverse (uncompute circ targ) st
 
-//let tmp = assert(forall st x. Equal (applyGate st x) st)
+//let tmp = assert(forall st x. equal (applyGate st x) st)
