src/SetExtra.fst
@@ -1,0 +1,67 @@
+(** Extra set operations *)
+module SetExtra
+open FStar.Set
+
+val full         : #a:eqtype -> Tot (set a)
+val diff         : #a:eqtype -> set a -> set a -> Tot (set a)
+val symdiff      : #a:eqtype -> set a -> set a -> Tot (set a)
+val ins          : #a:eqtype -> a -> set a -> Tot (set a)
+val rem          : #a:eqtype -> a -> set a -> Tot (set a)
+
+(* This is poor design. Computational sets are needed elsewhere... *)
+val fold : #a:eqtype -> #b:eqtype -> (b -> a -> b) -> b -> set a -> b
+let fold #a #b f b s = admit()
+
+let full #a         = complement (empty #a)
+let diff #a s s'    = intersect s (complement s')
+let symdiff #a s s' = diff (union s s') (intersect s s')
+let ins #a x s      = union (singleton x) s 
+let rem #a x s      = diff s (singleton x)
+
+(** Verification utilities *)
+
+(* Subset relation & lemmas *)
+type disjoint (#a:eqtype) (s:set a) (s':set a) = forall x. ~(mem x s /\ mem x s')
+
+val subset_trans : #a:eqtype -> s:set a -> s':set a -> s'':set a ->
+  Lemma (requires (subset s s' /\ subset s' s''))
+        (ensures  (subset s s''))
+let subset_trans #a s s' s'' = ()
+
+val subset_ins : #a:eqtype -> x:a -> s:set a ->
+  Lemma (subset s (ins x s))
+let subset_ins #a x s = ()
+
+val ins_rem_equal : #a:eqtype -> x:a -> s:set a ->
+  Lemma (requires True)
+	(ensures (ins x (rem x s) == (ins x s)))
+  [SMTPat (ins x (rem x s))]
+let ins_rem_equal #a x s =
+  lemma_equal_intro (ins x (rem x s)) (ins x s)
+
+val ins_subset_pres : #a:eqtype -> x:a -> s:set a -> s':set a ->
+  Lemma (requires (subset s s'))
+        (ensures  (subset (ins x s) (ins x s')))
+let ins_subset_pres #a x s s' = ()
+
+val disjoint_subset : #a:eqtype -> s:set a -> s':set a -> s'':set a ->
+  Lemma (requires (subset s s' /\ disjoint s' s''))
+        (ensures  (disjoint s s''))
+let disjoint_subset #a s s' s'' = ()
+
+val disjoint_union : #a:eqtype -> s:set a -> s':set a -> s'':set a ->
+  Lemma (requires (disjoint s s' /\ disjoint s s''))
+        (ensures  (disjoint s (union s' s'')))
+let disjoint_union #a s s' s'' = ()
+
+val disjoint_is_subset_compl : #a:eqtype -> s:set a -> s':set a ->
+  Lemma (disjoint s s' <==> subset s (complement s'))
+let disjoint_is_subset_compl #a s s' = ()
+
+val subset_compl_reverse : #a:eqtype -> s:set a -> s':set a ->
+  Lemma (subset s s' <==> subset (complement s') (complement s))
+let subset_compl_reverse #a s s' = ()
+
+val union_equal : #a:eqtype ->
+  Lemma (equal (empty #a) (union (empty #a) (empty #a)))
+let union_equal #a = ()
